src/HOL/Induct/Com.thy
@@ -5,7 +5,7 @@
 Example of Mutual Induction via Iteratived Inductive Definitions: Commands
 *)
 
-section{*Mutual Induction via Iteratived Inductive Definitions*}
+section\<open>Mutual Induction via Iteratived Inductive Definitions\<close>
 
 theory Com imports Main begin
 
@@ -25,15 +25,15 @@ and
       | While exp com          ("WHILE _ DO _"  60)
 
 
-subsection {* Commands *}
+subsection \<open>Commands\<close>
 
-text{* Execution of commands *}
+text\<open>Execution of commands\<close>
 
 abbreviation (input)
   generic_rel  ("_/ -|[_]-> _" [50,0,50] 50)  where
   "esig -|[eval]-> ns == (esig,ns) \<in> eval"
 
-text{*Command execution.  Natural numbers represent Booleans: 0=True, 1=False*}
+text\<open>Command execution.  Natural numbers represent Booleans: 0=True, 1=False\<close>
 
 inductive_set
   exec :: "((exp*state) * (nat*state)) set => ((com*state)*state)set"
@@ -74,7 +74,7 @@ inductive_cases
     and exec_WHILE_case: "(WHILE b DO c,s) -[eval]-> t"
 
 
-text{*Justifies using "exec" in the inductive definition of "eval"*}
+text\<open>Justifies using "exec" in the inductive definition of "eval"\<close>
 lemma exec_mono: "A<=B ==> exec(A) <= exec(B)"
 apply (rule subsetI)
 apply (simp add: split_paired_all)
@@ -92,7 +92,7 @@ lemma [pred_set_conv]:
   unfolding subset_eq
   by (auto simp add: le_fun_def)
 
-text{*Command execution is functional (deterministic) provided evaluation is*}
+text\<open>Command execution is functional (deterministic) provided evaluation is\<close>
 theorem single_valued_exec: "single_valued ev ==> single_valued(exec ev)"
 apply (simp add: single_valued_def)
 apply (intro allI)
@@ -102,9 +102,9 @@ apply (blast elim: exec_WHILE_case)+
 done
 
 
-subsection {* Expressions *}
+subsection \<open>Expressions\<close>
 
-text{* Evaluation of arithmetic expressions *}
+text\<open>Evaluation of arithmetic expressions\<close>
 
 inductive_set
   eval    :: "((exp*state) * (nat*state)) set"
@@ -136,13 +136,13 @@ lemma var_assign_eval [intro!]: "(X x, s(x:=n)) -|-> (n, s(x:=n))"
   by (rule fun_upd_same [THEN subst]) fast
 
 
-text{* Make the induction rule look nicer -- though @{text eta_contract} makes the new
-    version look worse than it is...*}
+text\<open>Make the induction rule look nicer -- though @{text eta_contract} makes the new
+    version look worse than it is...\<close>
 
 lemma split_lemma: "{((e,s),(n,s')). P e s n s'} = Collect (split (%v. split (split P v)))"
   by auto
 
-text{*New induction rule.  Note the form of the VALOF induction hypothesis*}
+text\<open>New induction rule.  Note the form of the VALOF induction hypothesis\<close>
 lemma eval_induct
   [case_names N X Op valOf, consumes 1, induct set: eval]:
   "[| (e,s) -|-> (n,s');
@@ -167,12 +167,12 @@ apply (auto simp add: split_lemma)
 done
 
 
-text{*Lemma for @{text Function_eval}.  The major premise is that @{text "(c,s)"} executes to @{text "s1"}
+text\<open>Lemma for @{text Function_eval}.  The major premise is that @{text "(c,s)"} executes to @{text "s1"}
   using eval restricted to its functional part.  Note that the execution
   @{text "(c,s) -[eval]-> s2"} can use unrestricted @{text eval}!  The reason is that
   the execution @{text "(c,s) -[eval Int {...}]-> s1"} assures us that execution is
   functional on the argument @{text "(c,s)"}.
-*}
+\<close>
 lemma com_Unique:
  "(c,s) -[eval Int {((e,s),(n,t)). \<forall>nt'. (e,s) -|-> nt' --> (n,t)=nt'}]-> s1
   ==> \<forall>s2. (c,s) -[eval]-> s2 --> s2=s1"
@@ -190,7 +190,7 @@ apply (erule exec_WHILE_case, blast+)
 done
 
 
-text{*Expression evaluation is functional, or deterministic*}
+text\<open>Expression evaluation is functional, or deterministic\<close>
 theorem single_valued_eval: "single_valued eval"
 apply (unfold single_valued_def)
 apply (intro allI, rule impI)
@@ -204,14 +204,14 @@ done
 lemma eval_N_E [dest!]: "(N n, s) -|-> (v, s') ==> (v = n & s' = s)"
   by (induct e == "N n" s v s' set: eval) simp_all
 
-text{*This theorem says that "WHILE TRUE DO c" cannot terminate*}
+text\<open>This theorem says that "WHILE TRUE DO c" cannot terminate\<close>
 lemma while_true_E:
     "(c', s) -[eval]-> t ==> c' = WHILE (N 0) DO c ==> False"
   by (induct set: exec) auto
 
 
-subsection{* Equivalence of IF e THEN c;;(WHILE e DO c) ELSE SKIP  and
-       WHILE e DO c *}
+subsection\<open>Equivalence of IF e THEN c;;(WHILE e DO c) ELSE SKIP  and
+       WHILE e DO c\<close>
 
 lemma while_if1:
      "(c',s) -[eval]-> t
@@ -233,8 +233,8 @@ by (blast intro: while_if1 while_if2)
 
 
 
-subsection{* Equivalence of  (IF e THEN c1 ELSE c2);;c
-                         and  IF e THEN (c1;;c) ELSE (c2;;c)   *}
+subsection\<open>Equivalence of  (IF e THEN c1 ELSE c2);;c
+                         and  IF e THEN (c1;;c) ELSE (c2;;c)\<close>
 
 lemma if_semi1:
      "(c',s) -[eval]-> t
@@ -254,9 +254,9 @@ theorem if_semi: "(((IF e THEN c1 ELSE c2);;c, s) -[eval]-> t)  =
 
 
 
-subsection{* Equivalence of  VALOF c1 RESULTIS (VALOF c2 RESULTIS e)
+subsection\<open>Equivalence of  VALOF c1 RESULTIS (VALOF c2 RESULTIS e)
                   and  VALOF c1;;c2 RESULTIS e
- *}
+\<close>
 
 lemma valof_valof1:
      "(e',s) -|-> (v,s')
@@ -276,7 +276,7 @@ theorem valof_valof:
   by (blast intro: valof_valof1 valof_valof2)
 
 
-subsection{* Equivalence of  VALOF SKIP RESULTIS e  and  e *}
+subsection\<open>Equivalence of  VALOF SKIP RESULTIS e  and  e\<close>
 
 lemma valof_skip1:
      "(e',s) -|-> (v,s')
@@ -293,7 +293,7 @@ theorem valof_skip:
   by (blast intro: valof_skip1 valof_skip2)
 
 
-subsection{* Equivalence of  VALOF x:=e RESULTIS x  and  e *}
+subsection\<open>Equivalence of  VALOF x:=e RESULTIS x  and  e\<close>
 
 lemma valof_assign1:
      "(e',s) -|-> (v,s'')
